\documentclass[a4paper]{article}
\usepackage{geometry}
 \geometry{
 a4paper,
 total={170mm,257mm},
 left=20mm,
 top=20mm,
 }

\usepackage[english]{babel}
\usepackage[utf8]{inputenc}
\usepackage{amsmath}
\usepackage{bm}
\usepackage{graphicx,wrapfig,lipsum}

\usepackage[colorinlistoftodos]{todonotes}
\usepackage{hyperref}






\usepackage{enumitem}
\newcommand{\subscript}[2]{$#1 _ #2$}
\usepackage{listings}
 \usepackage{xcolor}



\hypersetup{
    colorlinks=true,
    linkcolor=blue,
    filecolor=magenta,      
    urlcolor=red,
    pdftitle={An Example},
    pdfpagemode=FullScreen,
    }
\urlstyle{same}


\def\ba{\begin{eqnarray}}
\def\ea{\end{eqnarray}}


\title{ Euclid summer school: Parameter estimation for a polynomial model}

\begin{document}

\maketitle


\section{Analytical solution}

1) 

\ba
{\cal L}( \{d_{i} \} | \{a_{k} \}) &=& \frac{1}{(2\pi)^{N/2} \sqrt{\rm  det \ \Sigma} } {\rm exp}  - \frac{1}{2} \left[ \sum_{ij} \left( d_{i}  -\sum_{k=0}^{M} a_{k}  (z_{i}-z_{c})^{k} \right)    \Sigma_{ij}^{-1}  \left( d_{j}  -\sum_{\ell=0}^{M} a_{\ell}  (z_{j}-z_{c})^{\ell} \right)  \right]  \nonumber \\
&=& \frac{1}{(2\pi)^{N/2} \sqrt{\rm  det \ \Sigma} } {\rm exp}  - \frac{1}{2} \left[  \left( \bm{d} - {\cal P} \bm{a} \right)^{T}    \Sigma^{-1}  \left( \bm{d} - {\cal P} \bm{a} \right)  \right]
\ea

5)

\ba
{\rm ln}{\cal L}(\bm{d} | \bm{a}) &=& -\frac{N}{2} {\rm ln}(2\pi) - \frac{1}{2} \ln ({\rm det}( \Sigma)) -\frac{1}{2} \left[ ( \bm{d} - {\cal P}\bm{a})^{T} \Sigma^{-1}   ( \bm{d} - {\cal P}\bm{a})\right]  \nonumber \\
\frac{\partial{\rm ln}{\cal L}(\bm{d} | \bm{a})}{\partial a_{\gamma}}Â  &=&   - \frac{1}{2} \sum_{ij} \left[ (  \sum_{\alpha}{\cal P}_{i\alpha}\delta_{\alpha\gamma}) (\Sigma^{-1})_{ij}   ( \bm{d}_{j} - \sum_{\beta}{\cal P}_{j\beta}\bm{a}_{\beta}) + ( \bm{d}_{i} - \sum_{\alpha}{\cal P}_{i\alpha}\bm{a}_{\alpha}) (\Sigma^{-1})_{ij}  \sum_{\beta}{\cal P}_{j\beta} \delta_{\beta\gamma} \right]   \nonumber \nonumber \\
&=&   - \frac{1}{2} \sum_{ij} \left[ (  {\cal P}_{i\gamma}) (\Sigma^{-1})_{ij}   ( \bm{d}_{j} - \sum_{\beta}{\cal P}_{j\beta}\bm{a}_{\beta}) + ( \bm{d}_{i} - \sum_{\alpha}{\cal P}_{i\alpha}\bm{a}_{\alpha}) (\Sigma^{-1})_{ij}  {\cal P}_{j\gamma} \right]   \nonumber \\
&=&  -  \sum_{ij}  (  {\cal P}_{i\gamma}) (\Sigma^{-1})_{ij}   ( \bm{d}_{j} - \sum_{\beta}{\cal P}_{j\beta}\bm{a}_{\beta})  
\ea
Where we used  the fact that the covariance matrix is symmetric
\ba
\bm{\nabla}_{\bm{a}} {\rm ln}{\cal L}(\bm{d} | \bm{a}) = - {\cal P}^{T}  \Sigma^{-1}( \bm{d} - {\cal P}\bm{a}) = 0   \\
 {\cal P}^{T}  \Sigma^{-1}{\cal P}\bm{\hat{a}} = {\cal P}^{T}  \Sigma^{-1} \bm{d} \nonumber  \\
    \bm{\hat{a}} = ( {\cal P}^{T}  \Sigma^{-1}{\cal P})^{-1}{\cal P}^{T}  \Sigma^{-1} \bm{d} 
\ea

6)

\ba
\langle  \bm{\hat{a}}  \rangle= ( {\cal P}^{T}  \Sigma^{-1}{\cal P})^{-1}{\cal P}^{T}  \Sigma^{-1} \langle \bm{d} \rangle =  ( {\cal P}^{T}  \Sigma^{-1}{\cal P})^{-1}{\cal P}^{T}  \Sigma^{-1} \langle  {\cal P}\bm{a} + \bm{n} \rangle  = \bm{a}
\ea
since $\langle  \bm{n} \rangle=0$
\ba
\langle  \bm{\hat{a}} \bm{\hat{a}}^{T}  \rangle &=& ( {\cal P}^{T}  \Sigma^{-1}{\cal P})^{-1}{\cal P}^{T}  \Sigma^{-1} \langle \bm{d}  \bm{d}^{T} \rangle  \Sigma^{-1}{\cal P} ( {\cal P}^{T}  \Sigma^{-1}{\cal P})^{-1} \nonumber \\
&=&  ( {\cal P}^{T}  \Sigma^{-1}{\cal P})^{-1}{\cal P}^{T}  \Sigma^{-1} \langle  ({\cal P}\bm{a} + \bm{n})({\cal P}\bm{a} + \bm{n})^{T}\rangle  \Sigma^{-1}{\cal P} ( {\cal P}^{T}  \Sigma^{-1}{\cal P})^{-1} \nonumber \\
&=&  ( {\cal P}^{T}  \Sigma^{-1}{\cal P})^{-1}{\cal P}^{T}  \Sigma^{-1}   {\cal P}\bm{a} \bm{a}^{T} {\cal P}^{T}   \Sigma^{-1}{\cal P} ( {\cal P}^{T}  \Sigma^{-1}{\cal P})^{-1} \nonumber \\
&+& ( {\cal P}^{T}  \Sigma^{-1}{\cal P})^{-1}{\cal P}^{T}  \Sigma^{-1} \Sigma  \Sigma^{-1}{\cal P} ( {\cal P}^{T}  \Sigma^{-1}{\cal P})^{-1} \nonumber \\
&=&   \bm{a} \bm{a}^{T}   +  ( {\cal P}^{T}  \Sigma^{-1}{\cal P})^{-1} \nonumber \\
{\rm Cov}(\bm{\hat{a}}) &=&  ( {\cal P}^{T}  \Sigma^{-1}{\cal P})^{-1}
\ea






\end{document}